src/goose_lang/recovery_adequacy.v
@@ -9,9 +9,9 @@ From Perennial.goose_lang Require Import typing adequacy lang crash_borrow.
 Set Default Proof Using "Type".
 
 Theorem goose_recv_adequacy `{ffi_sem: ffi_semantics} `{!ffi_interp ffi} {Hffi_adequacy:ffi_interp_adequacy} Σ `{hPre: !gooseGpreS Σ} s e r σ g φ φr φinv Φinv n :
-  ffi_initgP g → ffi_initP σ.(world) g →
+  ffi_initgP g.(global_world) → ffi_initP σ.(world) g.(global_world) →
   (∀ `(Hheap : !heapGS Σ),
-     ⊢ (ffi_global_start goose_ffiGlobalGS g -∗
+     ⊢ (ffi_global_start goose_ffiGlobalGS g.(global_world) -∗
         ffi_local_start goose_ffiLocalGS σ.(world) -∗
         trace_frag σ.(trace) -∗
         oracle_frag σ.(oracle) -∗
@@ -27,7 +27,7 @@ Proof.
   eapply (wp_recv_adequacy_inv Σ _ _ (n * 4 + crash_borrow_ginv_number)).
   iIntros (???).
   iMod (na_heap_name_init tls σ.(heap)) as (name_na_heap) "Hh".
-  iMod (ffi_global_init _ _ g) as (ffi_namesg) "(Hgw&Hgstart)"; first by eauto.
+  iMod (ffi_global_init _ _ g.(global_world)) as (ffi_namesg) "(Hgw&Hgstart)"; first by eauto.
   iMod (ffi_local_init _ _ σ.(world)) as (ffi_names) "(Hw&Hstart)"; first by eauto.
   iMod (trace_name_init σ.(trace) σ.(oracle)) as (name_trace) "(Htr&Htrfrag&Hor&Hofrag)".
   iMod (credit_name_init (n*4 + crash_borrow_ginv_number)) as (name_credit) "(Hcred_auth&Hcred&Htok)".
